

7

$$16. (1). \cos A = \frac{b^2 + c^2 - a^2}{2bc} = \frac{\sqrt{2}}{2}$$

$$\frac{1}{2}c^2 = b^2 - a^2$$

$$c^2 = a^2 + b^2 - 2ab \cos C$$

$$\sin B - \sin^2 A = \pm \sin^2 C$$

$$\sin^2 A \cos^2 C + \pm \sin 2A \cdot \pm \sin 2C + \pm \sin 2C \cdot \pm \sin 2A + \sin^2 A \cos^2 A$$

$$-\sin^2 A = \pm \sin^2 C$$

$$\frac{1}{2} \cos^2 C + \frac{1}{2} \sin 2C + \frac{1}{2} \cos^2 C \pm \sin^2 C - \frac{1}{2} = \pm \sin^2 C$$

$$\cos^2 C + \sin 2C + \sin^2 C - 1 = \sin^2 C$$

$$\cos^2 C + 1 - 2\sin^2 C + \sin^2 C - 1 = \sin^2 C$$

$$\cos^2 C = 2\sin^2 C$$

$$\therefore \frac{\sin^2 C}{\cos^2 C} = \frac{1}{2} \quad \therefore \tan C = \pm \frac{1}{\sqrt{2}} \quad \therefore \tan C = \frac{\sqrt{2}}{2}$$

$$12) \sin C = \frac{\sqrt{2}}{3} \quad \cos C = \frac{\sqrt{7}}{3}$$

$$\sin B = \sin(A+C) = \sin A \cos C + \cos A \sin C$$

$$= \frac{\sqrt{2}}{2} \cdot \frac{\sqrt{7}}{3} + \frac{\sqrt{3}}{2} \cdot \frac{\sqrt{2}}{3} = \frac{2\sqrt{6} + \sqrt{3}}{6}$$

$$S_{\triangle ABC} = \frac{1}{2} bc \sin A = 3$$

$$bc = 6\sqrt{2}$$

$$a^2 = b^2 + c^2 - 2bc \cos A$$

$$\therefore b = 2\sqrt{2}$$

AI Response:

€ • , f

„ ... † ‡ ^

% Š<

1. **Œ• **^

- ž • • ' ' " " • — — ~ ™ A " " š > œ €

- • , — ž Ÿ ¡ ™ € £ ¤ ¥ ¦ § ¨ © ª « » œ ¬ - ® - €

2. ** **^

- Œ• - ° ± • ' ' ² $\frac{1}{2}$ ³ > ª Ÿ ´ μ ¶ © . © > ¹ º «
» ¼ ¤ £ « ¬ ½¾ ¿ Ä Œ• - Á Â Ã • ½œ¬ Ä Å Æ €

- Ç È œ É • ½¾ $\tan C = \frac{\sqrt{3}}{2}$ μ ¶ Ê ¾ f Ë Ì ¿ À
Í Î Ï Ë Ì œ¬ • ½ Ð Ä Å Ñ €

% Ò Š<

1. **Œ• **^

- ž Ó Ô \$ \sin C\$ \$ \cos C\$ š Õ œ ~ \$ \sin B\$ > œ €

- • Ö • ' ¡ ™ × Ø Ù ° « Œ• \$ \Delta_{ABC}\$ Ø Ù Ú ½¾ \$ bc=6\sqrt{2}\$ > œ
- €

- Ç È ž " " • — ~ Û Ü \$ b\$ ½¾ \$ b=2\sqrt{2}\$ > œ - €

2. ** **^

- Œ• \$ \sin B\$ Ý É • Ê ¾ ' Þ ß μ ¶ Ĩ à á Œ• ¿ À Í Î Ĩ Œ• œ
¬ • ½ Ð Ä Å Ñ €

- Ç È œ ~ Û Ü \$ b\$ Ý É • Ê ¾ ' Þ ß μ ¶ Ĩ à á Œ• ¿ À Í Î Ĩ
Œ• œ¬ • ½ Ð Ä Å Ñ €

â ® ã ä

 Œ• - ¿ À Œ•
- Á Â Ã Ĩ Ë Ì œ¬ • ½ Ð Ä Å Ñ € å Ý ¿ À
- æ † Œ• ç è è é ê ¾ ë ì í î ï €